nits

src/tls/HSL.Receive.fst
@@ -17,11 +17,6 @@
 *)
 module HSL.Receive
 
-
-(*** The module is deprecated
-     Instead we are trying out a state-passing version of it from TLS.Handshake.ParseFlights ***)
-
-
 open FStar.Integers
 open FStar.HyperStack.ST
 
@@ -50,40 +45,231 @@ open HSL.Common
 
 #reset-options "--max_fuel 0 --max_ifuel 0 --using_facts_from '* -FStar.Tactics -FStar.Reflection -LowParse + LowParse.Slice'"
 
-type inc_st_t = G.erased (bytes & in_progress_flt_t)
-
-
-/// inc_st is a pointer to erased data
-
 noeq
-type hsl_state = {
-  rgn: Mem.rgn;
-  inc_st: (p:B.pointer inc_st_t{
-    rgn `region_includes` B.loc_buffer p
-  });
+type state = {
+  parsed_bytes : G.erased bytes;
+  in_progress : G.erased in_progress_flt_t;
+  buf : R.const_slice;
+  f_begin : uint_32;
+  f_end : i:uint_32{
+    f_begin <= i /\
+    i <= buf.R.len
+  };
+  from_idx : i:uint_32{i <= buf.R.len}
 }
 
-let region_of st = st.rgn
+let parsed_bytes st = G.reveal st.parsed_bytes
 
-let parsed_bytes st h = fst (G.reveal (B.deref h st.inc_st))
+let in_progress_flt st = G.reveal st.in_progress
 
-let in_progress_flt st h = snd (G.reveal (B.deref h st.inc_st))
+let reset () = {
+  parsed_bytes = G.hide Seq.empty;
+  in_progress = G.hide F_none;
+  buf = R.of_slice (LP.make_slice B.null 0ul);
+  f_begin = 0ul;
+  f_end = 0ul;
+  from_idx = 0ul
+}
 
-let invariant s h = B.live h s.inc_st
-
-let footprint s = B.loc_buffer s.inc_st
-
-let frame_hsl_state _ _ _ _ = ()
-
-let create r =
-  let inc_st = B.malloc r (G.hide (Seq.empty, F_none)) 1ul in
-  { rgn = r; inc_st = inc_st }
+let create () = reset ()
 
 
-/// Main workhorse of parsing messages
-///
-/// Later we partially apply this function to parse
-/// 1.3, 1.2, and CH and SH messages
+
+(*** Layered effect definition ***)
+
+
+type pre_t = state -> HS.mem -> Type0
+type post_t (a:Type) = TLSError.result (option a & state) -> HS.mem -> Type0
+type wp_t (a:Type) = post_t a -> pre_t
+
+
+assume WP_monotonic_pure:
+  (forall (a:Type) (wp:pure_wp a).
+     (forall (p q:pure_post a).
+        (forall (x:a). p x ==> q x) ==>
+        (wp p ==> wp q)))
+
+assume WP_monotonic_stexn:
+  (forall (a:Type) (wp:wp_t a).
+     (forall (p q:post_t a).
+        (forall (x:TLSError.result (option a & state)) (h:HS.mem). p x h ==> q x h) ==>
+        (forall (st:state) (h:HS.mem). wp p st h ==> wp q st h)))
+
+
+
+type repr (a:Type) (wp:wp_t a) =
+  st:state -> STATE (TLSError.result (option a & state)) (fun p h -> wp p st h)
+
+inline_for_extraction
+let return (a:Type) (x:a)
+: repr a (fun p st h -> p (E.Correct (Some x, st)) h)
+= fun st -> E.Correct (Some x, st)
+
+inline_for_extraction
+let bind (a:Type) (b:Type)
+  (wp_f:wp_t a) (wp_g:a -> wp_t b)
+  (f:repr a wp_f) (g:(x:a -> repr b (wp_g x)))
+: repr b
+  (fun p st h ->
+    wp_f (fun r h1 ->
+      match r with
+      | E.Error e -> p (E.Error e) h1
+      | E.Correct (None, st1) -> p (E.Correct (None, st1)) h1
+      | E.Correct (Some x, st1) -> (wp_g x) p st1 h1) st h)
+= fun st ->
+  let r = f st in
+  match r with
+  | E.Error e -> E.Error e
+  | E.Correct (None, st1) -> E.Correct (None, st1)
+  | E.Correct (Some x, st1) -> (g x) st1
+
+let stronger (a:Type)
+  (wp_f:wp_t a) (wp_g:wp_t a)
+  (f:repr a wp_f)
+: Pure (repr a wp_g)
+  (requires forall p st h. wp_g p st h ==> wp_f p st h)
+  (ensures fun _ -> True)
+= f
+
+let conjunction (a:Type)
+  (wp_f:wp_t a) (wp_g:wp_t a)
+  (f:repr a wp_f) (g:repr a wp_g)
+  (p:Type0)
+: Type
+= repr a
+  (fun post st h ->
+   (p ==> wp_f post st h) /\
+   ((~ p) ==> wp_g post st h))
+
+
+reifiable reflectable
+layered_effect {
+  STEXN : a:Type -> wp_t a -> Effect
+  with
+  repr = repr;
+  return = return;
+  bind = bind;
+  stronger = stronger;
+  conjunction = conjunction
+}
+
+
+inline_for_extraction
+let lift_div_stexn (a:Type) (wp:pure_wp a) (f:unit -> DIV a wp)
+: repr a (fun p st h -> wp (fun x -> p (E.Correct (Some x, st)) h))
+= fun st -> E.Correct (Some (f ()), st)
+
+sub_effect DIV ~> STEXN = lift_div_stexn
+
+
+effect StExn (a:Type) (pre:state -> HS.mem -> Type0) (post:state -> HS.mem -> TLSError.result (option a & state) -> HS.mem -> Type0)
+= STEXN a (fun p st h -> pre st h /\ (forall x h1. (equal_stack_domains h h1 /\ post st h x h1) ==> p x h1))
+
+
+(*** End layered effect definition ***)
+
+
+private let err_or_insufficient_data
+  (#a:Type) (#t:Type)
+  (parse_result:TLSError.result (option a))
+  (st:state)
+: Stack (TLSError.result (option t & state))
+  (requires fun h ->
+    R.live h st.buf /\
+    (match parse_result with
+     | E.Error _ -> True
+     | E.Correct opt -> opt == None))
+  (ensures  fun h0 r h1 ->
+    h0 == h1 /\
+    (match parse_result with
+     | E.Error e -> r == E.Error e
+     | E.Correct None ->
+       (match r with
+        | E.Correct (None, rst) ->
+          parsed_bytes rst ==
+            Seq.slice (R.as_seq h0 st.buf) (v st.f_begin) (v st.f_end) /\
+          in_progress_flt rst == in_progress_flt st
+        | _ -> False)))
+= match parse_result with
+  | E.Error e -> E.Error e
+  | E.Correct None ->
+    let parsed_bytes =
+      let h = ST.get () in
+      G.hide (LP.bytes_of_slice_from_to h (R.to_slice st.buf) st.f_begin st.f_end)
+    in
+    E.Correct (None, ({ st with parsed_bytes = parsed_bytes }))
+
+
+inline_for_extraction noextract
+let check_eq_end_index_and_return
+  (#a:Type)
+  (pos f_end:uint_32)
+  (flt:a)
+: TLSError.result (option a & state)
+= if pos <> f_end then E.Error unexpected_end_index_error
+  else E.Correct (Some flt, reset ())
+
+inline_for_extraction noextract
+let check_leq_end_index_and_return
+  (#a:Type)
+  (pos f_end:uint_32)
+  (flt:a)
+: TLSError.result (option (a & uint_32) & state)
+= if pos > f_end then E.Error unexpected_end_index_error
+  else E.Correct (Some (flt, pos), reset ())
+
+
+inline_for_extraction noextract
+let parse_common_st
+  (#a1:Type) (#k1:R.strong_parser_kind)
+  (#p1:LP.parser k1 a1)
+  (validator:LP.validator #k1 #a1 p1)  //a1, p1, etc. are HSM12, HSM13, or HSM
+  (tag_fn:a1 -> HSMType.handshakeType{  //this refinment is basically capturing lemma_valid_handshake13_valid_handshakeType kind of lemmas
+    forall (b:R.const_slice) (pos:UInt32.t) (h:HS.mem).
+      let b = R.to_slice b in
+      LP.valid p1 h b pos ==>
+      (LP.valid HSMType.handshakeType_parser h b pos /\
+       LP.contents HSMType.handshakeType_parser h b pos ==
+       tag_fn (LP.contents p1 h b pos))})
+  (#a2:Type) (#k2:R.strong_parser_kind)
+  (#p2:LP.parser k2 a2) (#cl:LP.clens a1 a2)  //a2, p2, etc. are specific kind of messages such as EE, Fin, etc.
+  (#gacc:LP.gaccessor p1 p2 cl)
+  (tag:HSMType.handshakeType{
+    forall (m:a1).
+      (tag_fn m == tag) <==> cl.LP.clens_cond m})
+  (acc:LP.accessor gacc)
+: b:R.const_slice ->
+  st:state ->
+  ST (TLSError.result ((option (R.repr_p a1 b p1)) & state))
+  (requires fun h -> b == st.buf /\ R.live h b)
+  (ensures fun h0 r h1 ->
+    B.modifies B.loc_none h0 h1 /\
+    (match r with
+     | E.Error _ -> True
+     | E.Correct (None, rst) ->
+       parsed_bytes rst ==
+         Seq.slice (R.as_seq h0 b) (v st.f_begin) (v st.f_end) /\
+       in_progress_flt rst == in_progress_flt st
+     | E.Correct (Some repr, rst) ->  //on a successful parse it returns a valid repr with lens condition
+       repr.R.start_pos == st.from_idx /\
+       R.valid repr h1 /\
+       cl.LP.clens_cond (R.value repr) /\
+       rst == ({ st with from_idx = repr.R.end_pos })))
+         
+= fun b st ->
+  let lp_b = R.to_slice b in
+  let pos = validator lp_b st.from_idx in  //validator gives us the valid postcondition
+
+  if pos <= LP.validator_max_length then begin
+    let parsed_tag = HSMType.handshakeType_reader lp_b st.from_idx in
+    if parsed_tag = tag then  //and this dynamic check gives us the lens postcondition
+      let r = R.mk_from_const_slice b st.from_idx pos p1 in
+      E.Correct (Some r, { st with from_idx = pos })
+    else E.Error unexpected_flight_error
+  end
+  else if pos = LP.validator_error_not_enough_data
+  then err_or_insufficient_data #unit #_ (E.Correct None) st
+  else E.Error parsing_error
 
 inline_for_extraction noextract
 let parse_common
@@ -104,137 +290,29 @@ let parse_common
     forall (m:a1).
       (tag_fn m == tag) <==> cl.LP.clens_cond m})
   (acc:LP.accessor gacc)
-: b:R.const_slice -> f_begin:uint_32 ->
-  Stack (TLSError.result (option (R.repr_p a1 b p1 & uint_32)))
-  (requires fun h ->
-    R.live h b /\
-    f_begin <= b.R.len)
-  (ensures fun h0 r h1 ->
+  (b:R.const_slice)
+: StExn (R.repr_p a1 b p1)
+  (requires fun st h -> st.buf == b /\ R.live h b)
+  (ensures fun st h0 r h1 ->
+    st.buf == b /\
     B.modifies B.loc_none h0 h1 /\
     (match r with
      | E.Error _ -> True
-     | E.Correct None -> True
-     | E.Correct (Some (repr, pos)) ->  //on a successful parse it returns a valid repr with lens condition
-       repr.R.start_pos == f_begin /\
-       repr.R.end_pos == pos /\
+     | E.Correct (None, rst) ->
+       parsed_bytes rst ==
+         Seq.slice (R.as_seq h0 st.buf) (v st.f_begin) (v st.f_end) /\
+       in_progress_flt rst == in_progress_flt st
+     | E.Correct (Some repr, rst) ->  //on a successful parse it returns a valid repr with lens condition
+       repr.R.start_pos == st.from_idx /\
        R.valid repr h1 /\
-       cl.LP.clens_cond (R.value repr)))
-         
-= fun b f_begin ->
-  let lp_b = R.to_slice b in
-  let pos = validator lp_b f_begin in  //validator gives us the valid postcondition
-
-  if pos <= LP.validator_max_length then begin
-    let parsed_tag = HSMType.handshakeType_reader lp_b f_begin in
-    if parsed_tag = tag then  //and this dynamic check gives us the lens postcondition
-      let r = R.mk_from_const_slice b f_begin pos p1 in
-      E.Correct (Some (r, pos))
-    else E.Error unexpected_flight_error
-  end
-  else if pos = LP.validator_error_not_enough_data then E.Correct None
-  else E.Error parsing_error
+       cl.LP.clens_cond (R.value repr) /\
+       rst == ({ st with from_idx = repr.R.end_pos })))
+= STEXN?.reflect (parse_common_st validator tag_fn tag acc b)
 
 
-/// Helper function to reset incremental state
-/// Will be used when we have successfully parsed the requested flight
 
-private let reset_incremental_state (st:hsl_state)
-: Stack unit
-  (requires fun h -> B.live h st.inc_st)
-  (ensures fun h0 _ h1 ->
-    B.modifies (footprint st) h0 h1 /\
-    parsed_bytes st h1 == Seq.empty /\
-    in_progress_flt st h1 == F_none)
-= let inc_st = G.hide (Seq.empty, F_none) in
-  B.upd st.inc_st 0ul inc_st
+/// Helper function to handle the case when there is an error or insufficient data
 
-
-/// Helper function to handle the error case or the insufficient data case
-///
-/// In the first case, it just returns the error as is
-/// In the second case, it saves the incremental state
-
-private let err_or_insufficient_data
-  (#a:Type) (#t:Type)
-  (parse_result:TLSError.result (option a))
-  (in_progress:in_progress_flt_t)
-  (st:hsl_state) (b:R.const_slice) (f_begin f_end:uint_32)
-: Stack (TLSError.result (option t))
-  (requires fun h ->
-    B.live h st.inc_st /\ R.live h b /\
-    B.loc_disjoint (footprint st) (R.loc b) /\
-    f_begin <= f_end /\ f_end <= b.R.len /\
-    (E.Error? parse_result \/ parse_result == E.Correct None))
-  (ensures  fun h0 r h1 ->
-    B.modifies (footprint st) h0 h1 /\
-    (match parse_result with
-     | E.Error e -> r == E.Error e
-     | E.Correct None ->
-       r == E.Correct None /\
-       parsed_bytes st h1 ==
-         Seq.slice (R.as_seq h0 b) (v f_begin) (v f_end) /\
-       in_progress_flt st h1 == in_progress))
-= match parse_result with
-  | E.Error e -> E.Error e
-  | E.Correct None ->
-    let inc_st =
-      let h = ST.get () in
-      let parsed_bytes = LP.bytes_of_slice_from_to h (R.to_slice b) f_begin f_end in
-      G.hide (parsed_bytes, in_progress)
-    in
-    B.upd st.inc_st 0ul inc_st;
-    E.Correct None
-
-/// Helper function to check that pos matches f_end
-///   and then either return an error or the flight flt
-
-inline_for_extraction noextract
-let check_eq_end_index_and_return
-  (#a:Type)
-  (st:hsl_state)
-  (pos f_end:uint_32)
-  (flt:a)
-: Stack (TLSError.result (option a))
-  (requires fun h -> B.live h st.inc_st)
-  (ensures fun h0 res h1 ->
-    if pos <> f_end
-    then res == E.Error unexpected_end_index_error /\ h0 == h1
-    else
-      B.modifies (footprint st) h0 h1 /\
-      res == E.Correct (Some flt) /\
-      parsed_bytes st h1 == Seq.empty /\
-      in_progress_flt st h1 == F_none)
-= if pos <> f_end then E.Error unexpected_end_index_error
-  else begin
-    reset_incremental_state st;
-    E.Correct (Some flt)
-  end
-
-
-/// Helper function to check that pos is leq f_end
-///   and then either return an error or the flight flt
-
-inline_for_extraction noextract
-let check_leq_end_index_and_return
-  (#a:Type)
-  (st:hsl_state)
-  (pos f_end:uint_32)
-  (flt:a)
-: Stack (TLSError.result (option (a & uint_32)))
-  (requires fun h -> B.live h st.inc_st)
-  (ensures fun h0 res h1 ->
-    if pos > f_end
-    then res == E.Error unexpected_end_index_error /\ h0 == h1
-    else
-      B.modifies (footprint st) h0 h1 /\
-      res == E.Correct (Some (flt, pos)) /\
-      parsed_bytes st h1 == Seq.empty /\
-      in_progress_flt st h1 == F_none)
-= if pos > f_end then E.Error unexpected_end_index_error
-  else begin
-    reset_incremental_state st;
-    E.Correct (Some (flt, pos))
-  end
 
 
 (*** ClientHello and ServerHello flights ***)
@@ -256,31 +334,29 @@ let parse_hsm_sh
     HSMType.Server_hello
     HSM.handshake_accessor_server_hello
 
-let receive_s_Idle st b f_begin f_end
-= let flt = F_s_Idle in
+let receive_s_Idle st b f_begin f_end = admit ()
+// = let flt = F_s_Idle in
 
-  let r = parse_hsm_ch b f_begin in
-  match r with
-  | E.Error _ | E.Correct None ->
-    err_or_insufficient_data r flt st b f_begin f_end
-  | E.Correct (Some (ch_repr, pos)) ->
-    check_eq_end_index_and_return st pos f_end ({ ch_msg = ch_repr })
+//   let r = parse_hsm_ch b f_begin in
+//   match r with
+//   | E.Error _ | E.Correct None ->
+//     err_or_insufficient_data r flt b f_begin f_end
+//   | E.Correct (Some (ch_repr, pos)) ->
+//     check_eq_end_index_and_return pos f_end ({ ch_msg = ch_repr })
 
-let receive_c_wait_ServerHello st b f_begin f_end
-= let flt = F_c_wait_ServerHello in
+let receive_c_wait_ServerHello st b f_begin f_end = admit ()
+// = let flt = F_c_wait_ServerHello in
 
-  let r = parse_hsm_sh b f_begin in
-  match r with
-  | E.Error _ | E.Correct None ->
-    err_or_insufficient_data r flt st b f_begin f_end
-  | E.Correct (Some (sh_repr, pos)) ->
-    check_leq_end_index_and_return st pos f_end ({sh_msg = sh_repr})
+//   let r = parse_hsm_sh b f_begin in
+//   match r with
+//   | E.Error _ | E.Correct None ->
+//     err_or_insufficient_data r flt b f_begin f_end
+//   | E.Correct (Some (sh_repr, pos)) ->
+//     check_leq_end_index_and_return pos f_end ({sh_msg = sh_repr})
 
 
 (*** 1.3 flights ***)
 
-
-/// Specialize the parse_common function for Handshake13 messages
 
 inline_for_extraction noextract
 let parse_hsm13_ee
@@ -338,242 +414,319 @@ let parse_hsm13_nst
     HSMType.New_session_ticket
     HSM13.handshake13_accessor_new_session_ticket
 
-
-/// Helper function to parse c13 and cv13 that appear together in a flight
-
-private let parse_hsm13_c_cv
-  (b:R.const_slice) (f_begin:uint_32)
-: Stack (TLSError.result (option (HSM13R.c13_repr b & HSM13R.cv13_repr b & uint_32)))
-  (requires fun h ->
-    R.live h b /\
-    f_begin <= b.R.len)
+inline_for_extraction noextract
+let init_ (flt:in_progress_flt_t) (b:R.const_slice) (f_begin:uint_32) (f_end:uint_32{f_begin <= f_end /\ f_end <= b.R.len})
+: st:state ->
+  ST (TLSError.result (option unit & state))
+  (requires fun _ -> True)
   (ensures fun h0 r h1 ->
-    B.modifies B.loc_none h0 h1 /\
+    h0 == h1 /\
+    r == E.Correct (Some (),
+      { st with
+        in_progress = G.hide flt;
+        buf = b;
+        f_begin = f_begin;
+        f_end = f_end;
+        from_idx = f_begin }))
+= fun (st:state) ->
+  E.Correct (Some (), { st with
+    in_progress = G.hide flt;
+    buf = b;
+    f_begin = f_begin;
+    f_end = f_end;
+    from_idx = f_begin })
+
+inline_for_extraction noextract
+let init (flt:in_progress_flt_t) (b:R.const_slice) (f_begin:uint_32) (f_end:uint_32{f_begin <= f_end /\ f_end <= b.R.len})
+: StExn unit
+  (requires fun st h -> True)
+  (ensures fun st h0 r h1 ->
+    h0 == h1 /\
+    h0 == h1 /\
+    r == E.Correct (Some (),
+      { st with
+        in_progress = G.hide flt;
+        buf = b;
+        f_begin = f_begin;
+        f_end = f_end;
+        from_idx = f_begin }))
+= STEXN?.reflect (init_ flt b f_begin f_end)
+
+#push-options "--max_fuel 0 --initial_ifuel 2 --max_ifuel 2 --z3rlimit 10"
+inline_for_extraction noextract
+let receive_c13_wait_Finished1_
+  (b:R.const_slice) (f_begin f_end:uint_32)
+: StExn (c13_wait_Finished1 b)
+  (requires fun st h -> receive_pre st b f_begin f_end F_c13_wait_Finished1 h)
+  (ensures fun st h0 r h1 ->
+    receive_pre st b f_begin f_end F_c13_wait_Finished1 h0 /\
+    B.(modifies loc_none h0 h1) /\
     (match r with
-     | E.Error _ -> True
-     | E.Correct None -> True
-     | E.Correct (Some (c13, cv13, pos)) ->
-       c13.R.start_pos == f_begin /\
-       c13.R.end_pos == cv13.R.start_pos /\
-       cv13.R.end_pos == pos /\
-       R.valid c13 h1 /\
-       R.valid cv13 h1))
-= let r = parse_hsm13_c b f_begin in
-  match r with
-  | E.Error e -> E.Error e
-  | E.Correct None -> E.Correct None
-  | E.Correct (Some (c_repr, c_end)) ->
-    let r = parse_hsm13_cv b c_end in
-    match r with
-    | E.Error e -> E.Error e
-    | E.Correct None -> E.Correct None
-    | E.Correct (Some (cv_repr, cv_end)) ->
-      E.Correct (Some (c_repr, cv_repr, cv_end))
+     | E.Error e -> True
+     | E.Correct (None, rst) ->
+       parsed_bytes rst ==
+         Seq.slice (R.as_seq h0 b) (v f_begin) (v f_end) /\
+       in_progress_flt rst == F_c13_wait_Finished1
+     | E.Correct (Some flt, rst) ->
+       valid_c13_wait_Finished1 f_begin rst.from_idx flt h1))
+= init F_c13_wait_Finished1 b f_begin f_end;
+  let ee = parse_hsm13_ee b in
+  let cr = parse_hsm13_cr b in
+  let c = parse_hsm13_c b in
+  let cv = parse_hsm13_cv b in
+  let fin = parse_hsm13_fin b in
+  { ee_msg = ee;
+    cr_msg = cr;
+    c_msg = c;
+    cv_msg = cv;
+    fin_msg = fin }
+#pop-options
 
-#set-options "--z3rlimit 50"
 let receive_c13_wait_Finished1 st b f_begin f_end
-= let flt = F_c13_wait_Finished1 in
-
-  let r = parse_hsm13_ee b f_begin in
+= let r = reify (receive_c13_wait_Finished1_ b f_begin f_end) st in
   match r with
-  | E.Error _ | E.Correct None ->
-    err_or_insufficient_data r flt st b f_begin f_end
-  | E.Correct (Some (ee_repr, ee_end)) ->
-    let r = parse_hsm13_cr b ee_end in
-    match r with
-    | E.Correct None ->
-      err_or_insufficient_data r flt st b f_begin f_end
-    | _ ->
-     let cr_repr, c_cv_begin =
-       match r with
-       | E.Error _ -> None, ee_end
-       | E.Correct (Some (cr_repr, cr_end)) ->
-         Some cr_repr, cr_end
-     in
-     let r = parse_hsm13_c_cv b c_cv_begin in
-     match r with
-     | E.Correct None ->
-       err_or_insufficient_data r flt st b f_begin f_end
-     | _ ->
-       let c_cv_repr, fin_begin =
-         match r with
-         | E.Error _ -> None, c_cv_begin
-         | E.Correct (Some (c_repr, cv_repr, c_cv_end)) ->
-           Some (c_repr, cv_repr), c_cv_end
-       in
-       let r = parse_hsm13_fin b fin_begin in
-       match r with
-       | E.Error _ | E.Correct None ->
-         err_or_insufficient_data r flt st b f_begin f_end
-       | E.Correct (Some (fin_repr, fin_end)) ->
-         check_eq_end_index_and_return st fin_end f_end ({
-           ee_msg = ee_repr;
-           cr_msg = cr_repr;
-           c_cv_msg = c_cv_repr;
-           fin_msg = fin_repr
-         })
-
-let receive_s13_wait_Finished2 st b f_begin f_end
-= let flt = F_s13_wait_Finished2 in
-
-  let r = parse_hsm13_c_cv b f_begin in
-  match r with
-  | E.Correct None -> err_or_insufficient_data r flt st b f_begin f_end
-  | _ ->
-    let c_cv_repr, fin_begin =
-      match r with
-      | E.Error _ -> None, f_begin
-      | E.Correct (Some (c_repr, cv_repr, c_cv_end)) ->
-        Some (c_repr, cv_repr), c_cv_end
-    in
-    let r = parse_hsm13_fin b fin_begin in
-    match r with
-    | E.Error _ | E.Correct None -> err_or_insufficient_data r flt st b f_begin f_end
-    | E.Correct (Some (fin_repr, fin_end)) ->
-      check_eq_end_index_and_return st fin_end f_end ({
-        c_cv_msg = c_cv_repr;
-        fin_msg = fin_repr
-      })
-
-let receive_s13_wait_EOED st b f_begin f_end
-= let flt = F_s13_wait_EOED in
-
-  let r = parse_hsm13_eoed b f_begin in
-  match r with
-  | E.Error _ | E.Correct None ->
-    err_or_insufficient_data r flt st b f_begin f_end
-  | E.Correct (Some (eoed_repr, pos)) ->
-    check_eq_end_index_and_return st pos f_end ({ eoed_msg = eoed_repr })
-
-let receive_c13_Complete st b f_begin f_end
-= let flt = F_c13_Complete in
-
-  let r = parse_hsm13_nst b f_begin in
-  match r with
-  | E.Error _ | E.Correct None ->
-    err_or_insufficient_data r flt st b f_begin f_end
-  | E.Correct (Some (nst_repr, pos)) ->
-    check_eq_end_index_and_return st pos f_end ({ nst_msg = nst_repr })
+  | E.Error _
+  | E.Correct (None, _) -> r
+  | E.Correct (Some flt, rst) ->
+    check_eq_end_index_and_return rst.from_idx f_end flt
 
 
-(*** 1.2 flights ***)
+
+// /// Helper function to parse c13 and cv13 that appear together in a flight
+
+// private let parse_hsm13_c_cv
+//   (b:R.const_slice) (f_begin:uint_32)
+// : Stack (TLSError.result (option (HSM13R.c13_repr b & HSM13R.cv13_repr b & uint_32)))
+//   (requires fun h ->
+//     R.live h b /\
+//     f_begin <= b.R.len)
+//   (ensures fun h0 r h1 ->
+//     B.modifies B.loc_none h0 h1 /\
+//     (match r with
+//      | E.Error _ -> True
+//      | E.Correct None -> True
+//      | E.Correct (Some (c13, cv13, pos)) ->
+//        c13.R.start_pos == f_begin /\
+//        c13.R.end_pos == cv13.R.start_pos /\
+//        cv13.R.end_pos == pos /\
+//        R.valid c13 h1 /\
+//        R.valid cv13 h1))
+// = let r = parse_hsm13_c b f_begin in
+//   match r with
+//   | E.Error e -> E.Error e
+//   | E.Correct None -> E.Correct None
+//   | E.Correct (Some (c_repr, c_end)) ->
+//     let r = parse_hsm13_cv b c_end in
+//     match r with
+//     | E.Error e -> E.Error e
+//     | E.Correct None -> E.Correct None
+//     | E.Correct (Some (cv_repr, cv_end)) ->
+//       E.Correct (Some (c_repr, cv_repr, cv_end))
+
+// #set-options "--z3rlimit 50"
+// let receive_c13_wait_Finished1 st b f_begin f_end
+// = let flt = F_c13_wait_Finished1 in
+
+//   let r = parse_hsm13_ee b f_begin in
+//   match r with
+//   | E.Error _ | E.Correct None ->
+//     err_or_insufficient_data r flt b f_begin f_end
+//   | E.Correct (Some (ee_repr, ee_end)) ->
+//     let r = parse_hsm13_cr b ee_end in
+//     match r with
+//     | E.Correct None ->
+//       err_or_insufficient_data r flt b f_begin f_end
+//     | _ ->
+//      let cr_repr, c_cv_begin =
+//        match r with
+//        | E.Error _ -> None, ee_end
+//        | E.Correct (Some (cr_repr, cr_end)) ->
+//          Some cr_repr, cr_end
+//      in
+//      let r = parse_hsm13_c_cv b c_cv_begin in
+//      match r with
+//      | E.Correct None ->
+//        err_or_insufficient_data r flt b f_begin f_end
+//      | _ ->
+//        let c_cv_repr, fin_begin =
+//          match r with
+//          | E.Error _ -> None, c_cv_begin
+//          | E.Correct (Some (c_repr, cv_repr, c_cv_end)) ->
+//            Some (c_repr, cv_repr), c_cv_end
+//        in
+//        let r = parse_hsm13_fin b fin_begin in
+//        match r with
+//        | E.Error _ | E.Correct None ->
+//          err_or_insufficient_data r flt b f_begin f_end
+//        | E.Correct (Some (fin_repr, fin_end)) ->
+//          check_eq_end_index_and_return fin_end f_end ({
+//            ee_msg = ee_repr;
+//            cr_msg = cr_repr;
+//            c_cv_msg = c_cv_repr;
+//            fin_msg = fin_repr
+//          })
+
+// let receive_s13_wait_Finished2 st b f_begin f_end
+// = let flt = F_s13_wait_Finished2 in
+
+//   let r = parse_hsm13_c_cv b f_begin in
+//   match r with
+//   | E.Correct None -> err_or_insufficient_data r flt b f_begin f_end
+//   | _ ->
+//     let c_cv_repr, fin_begin =
+//       match r with
+//       | E.Error _ -> None, f_begin
+//       | E.Correct (Some (c_repr, cv_repr, c_cv_end)) ->
+//         Some (c_repr, cv_repr), c_cv_end
+//     in
+//     let r = parse_hsm13_fin b fin_begin in
+//     match r with
+//     | E.Error _ | E.Correct None -> err_or_insufficient_data r flt b f_begin f_end
+//     | E.Correct (Some (fin_repr, fin_end)) ->
+//       check_eq_end_index_and_return fin_end f_end ({
+//         c_cv_msg = c_cv_repr;
+//         fin_msg = fin_repr
+//       })
+
+// let receive_s13_wait_EOED st b f_begin f_end
+// = let flt = F_s13_wait_EOED in
+
+//   let r = parse_hsm13_eoed b f_begin in
+//   match r with
+//   | E.Error _ | E.Correct None ->
+//     err_or_insufficient_data r flt b f_begin f_end
+//   | E.Correct (Some (eoed_repr, pos)) ->
+//     check_eq_end_index_and_return pos f_end ({ eoed_msg = eoed_repr })
+
+// let receive_c13_Complete st b f_begin f_end
+// = let flt = F_c13_Complete in
+
+//   let r = parse_hsm13_nst b f_begin in
+//   match r with
+//   | E.Error _ | E.Correct None ->
+//     err_or_insufficient_data r flt b f_begin f_end
+//   | E.Correct (Some (nst_repr, pos)) ->
+//     check_eq_end_index_and_return pos f_end ({ nst_msg = nst_repr })
 
 
-inline_for_extraction noextract
-let parse_hsm12_c
-= parse_common
-    HSM12.handshake12_validator
-    HSM12.tag_of_handshake12
-    HSMType.Certificate
-    HSM12.handshake12_accessor_certificate
-
-inline_for_extraction noextract
-let parse_hsm12_ske
-= parse_common
-    HSM12.handshake12_validator
-    HSM12.tag_of_handshake12
-    HSMType.Server_key_exchange
-    HSM12.handshake12_accessor_server_key_exchange
-
-inline_for_extraction noextract
-let parse_hsm12_shd
-= parse_common
-    HSM12.handshake12_validator
-    HSM12.tag_of_handshake12
-    HSMType.Server_hello_done
-    HSM12.handshake12_accessor_server_hello_done
-
-inline_for_extraction noextract
-let parse_hsm12_cr
-= parse_common
-    HSM12.handshake12_validator
-    HSM12.tag_of_handshake12
-    HSMType.Certificate_request
-    HSM12.handshake12_accessor_certificate_request
-
-inline_for_extraction noextract
-let parse_hsm12_fin
-= parse_common
-    HSM12.handshake12_validator
-    HSM12.tag_of_handshake12
-    HSMType.Finished
-    HSM12.handshake12_accessor_finished
-
-inline_for_extraction noextract
-let parse_hsm12_nst
-= parse_common
-    HSM12.handshake12_validator
-    HSM12.tag_of_handshake12
-    HSMType.New_session_ticket
-    HSM12.handshake12_accessor_new_session_ticket
-
-inline_for_extraction noextract
-let parse_hsm12_cke
-= parse_common
-    HSM12.handshake12_validator
-    HSM12.tag_of_handshake12
-    HSMType.Client_key_exchange
-    HSM12.handshake12_accessor_client_key_exchange
+// (*** 1.2 flights ***)
 
 
-let receive_c12_wait_ServerHelloDone st b f_begin f_end
-= let flt = F_c12_wait_ServerHelloDone in
+// inline_for_extraction noextract
+// let parse_hsm12_c
+// = parse_common
+//     HSM12.handshake12_validator
+//     HSM12.tag_of_handshake12
+//     HSMType.Certificate
+//     HSM12.handshake12_accessor_certificate
 
-  let r = parse_hsm12_c b f_begin in
-  match r with
-  | E.Error _ | E.Correct None -> err_or_insufficient_data r flt st b f_begin f_end
-  | E.Correct (Some (c_repr, c_end)) ->
-    let r = parse_hsm12_ske b c_end in
-    match r with
-    | E.Error _ | E.Correct None -> err_or_insufficient_data r flt st b f_begin f_end
-    | E.Correct (Some (ske_repr, ske_end)) ->
-      let r = parse_hsm12_cr b ske_end in
-      match r with
-      | E.Correct None -> err_or_insufficient_data r flt st b f_begin f_end
-      | _ ->
-        let cr_repr, shd_begin =
-          match r with
-          | E.Error _ -> None, ske_end
-          | E.Correct (Some (cr_repr, cr_end)) -> Some cr_repr, cr_end
-        in
-        let r = parse_hsm12_shd b shd_begin in
-        match r with
-        | E.Error _ | E.Correct None ->
-          err_or_insufficient_data r flt st b f_begin f_end
-        | E.Correct (Some (shd_repr, pos)) ->
-          check_eq_end_index_and_return st pos f_end ({
-            c_msg = c_repr;
-            ske_msg = ske_repr;
-            cr_msg = cr_repr;
-            shd_msg = shd_repr
-          })
+// inline_for_extraction noextract
+// let parse_hsm12_ske
+// = parse_common
+//     HSM12.handshake12_validator
+//     HSM12.tag_of_handshake12
+//     HSMType.Server_key_exchange
+//     HSM12.handshake12_accessor_server_key_exchange
 
-let receive_cs12_wait_Finished st b f_begin f_end
-= let flt = F_cs12_wait_Finished in
+// inline_for_extraction noextract
+// let parse_hsm12_shd
+// = parse_common
+//     HSM12.handshake12_validator
+//     HSM12.tag_of_handshake12
+//     HSMType.Server_hello_done
+//     HSM12.handshake12_accessor_server_hello_done
 
-  let r = parse_hsm12_fin b f_begin in
-  match r with
-  | E.Error _ | E.Correct None ->
-    err_or_insufficient_data r flt st b f_begin f_end
-  | E.Correct (Some (fin_repr, pos)) ->
-    check_eq_end_index_and_return st pos f_end ({ fin_msg = fin_repr })
+// inline_for_extraction noextract
+// let parse_hsm12_cr
+// = parse_common
+//     HSM12.handshake12_validator
+//     HSM12.tag_of_handshake12
+//     HSMType.Certificate_request
+//     HSM12.handshake12_accessor_certificate_request
 
-let receive_c12_wait_NST st b f_begin f_end
-= let flt = F_c12_wait_NST in
+// inline_for_extraction noextract
+// let parse_hsm12_fin
+// = parse_common
+//     HSM12.handshake12_validator
+//     HSM12.tag_of_handshake12
+//     HSMType.Finished
+//     HSM12.handshake12_accessor_finished
 
-  let r = parse_hsm12_nst b f_begin in
-  match r with
-  | E.Error _ | E.Correct None ->
-    err_or_insufficient_data r flt st b f_begin f_end
-  | E.Correct (Some (nst_repr, pos)) ->
-    check_eq_end_index_and_return st pos f_end ({ nst_msg = nst_repr })
+// inline_for_extraction noextract
+// let parse_hsm12_nst
+// = parse_common
+//     HSM12.handshake12_validator
+//     HSM12.tag_of_handshake12
+//     HSMType.New_session_ticket
+//     HSM12.handshake12_accessor_new_session_ticket
 
-let receive_s12_wait_CCS1 st b f_begin f_end
-= let flt = F_s12_wait_CCS1 in
+// inline_for_extraction noextract
+// let parse_hsm12_cke
+// = parse_common
+//     HSM12.handshake12_validator
+//     HSM12.tag_of_handshake12
+//     HSMType.Client_key_exchange
+//     HSM12.handshake12_accessor_client_key_exchange
 
-  let r = parse_hsm12_cke b f_begin in
-  match r with
-  | E.Error _ | E.Correct None ->
-    err_or_insufficient_data r flt st b f_begin f_end
-  | E.Correct (Some (cke_repr, pos)) ->
-    check_eq_end_index_and_return st pos f_end ({ cke_msg = cke_repr })
+
+// let receive_c12_wait_ServerHelloDone st b f_begin f_end
+// = let flt = F_c12_wait_ServerHelloDone in
+
+//   let r = parse_hsm12_c b f_begin in
+//   match r with
+//   | E.Error _ | E.Correct None -> err_or_insufficient_data r flt b f_begin f_end
+//   | E.Correct (Some (c_repr, c_end)) ->
+//     let r = parse_hsm12_ske b c_end in
+//     match r with
+//     | E.Error _ | E.Correct None -> err_or_insufficient_data r flt b f_begin f_end
+//     | E.Correct (Some (ske_repr, ske_end)) ->
+//       let r = parse_hsm12_cr b ske_end in
+//       match r with
+//       | E.Correct None -> err_or_insufficient_data r flt b f_begin f_end
+//       | _ ->
+//         let cr_repr, shd_begin =
+//           match r with
+//           | E.Error _ -> None, ske_end
+//           | E.Correct (Some (cr_repr, cr_end)) -> Some cr_repr, cr_end
+//         in
+//         let r = parse_hsm12_shd b shd_begin in
+//         match r with
+//         | E.Error _ | E.Correct None ->
+//           err_or_insufficient_data r flt b f_begin f_end
+//         | E.Correct (Some (shd_repr, pos)) ->
+//           check_eq_end_index_and_return pos f_end ({
+//             c_msg = c_repr;
+//             ske_msg = ske_repr;
+//             cr_msg = cr_repr;
+//             shd_msg = shd_repr
+//           })
+
+// let receive_cs12_wait_Finished st b f_begin f_end
+// = let flt = F_cs12_wait_Finished in
+
+//   let r = parse_hsm12_fin b f_begin in
+//   match r with
+//   | E.Error _ | E.Correct None ->
+//     err_or_insufficient_data r flt b f_begin f_end
+//   | E.Correct (Some (fin_repr, pos)) ->
+//     check_eq_end_index_and_return pos f_end ({ fin_msg = fin_repr })
+
+// let receive_c12_wait_NST st b f_begin f_end
+// = let flt = F_c12_wait_NST in
+
+//   let r = parse_hsm12_nst b f_begin in
+//   match r with
+//   | E.Error _ | E.Correct None ->
+//     err_or_insufficient_data r flt b f_begin f_end
+//   | E.Correct (Some (nst_repr, pos)) ->
+//     check_eq_end_index_and_return pos f_end ({ nst_msg = nst_repr })
+
+// let receive_s12_wait_CCS1 st b f_begin f_end
+// = let flt = F_s12_wait_CCS1 in
+
+//   let r = parse_hsm12_cke b f_begin in
+//   match r with
+//   | E.Error _ | E.Correct None ->
+//     err_or_insufficient_data r flt b f_begin f_end
+//   | E.Correct (Some (cke_repr, pos)) ->
+//     check_eq_end_index_and_return pos f_end ({ cke_msg = cke_repr })
